Refactor the typing rules to use typed conversion

syntax.sig
@@ -1,17 +1,7 @@
 tm : Type
 nat : Type
 
-tAbs : (tm -> tm) -> tm
+tAbs : tm -> (tm -> tm) -> tm
 tApp : tm -> tm -> tm
 tPi : tm -> (tm -> tm) -> tm
 tUniv : nat -> tm
-tEq : tm -> tm -> tm -> tm
-tJ : tm -> tm -> tm -> tm -> tm
-tRefl : tm
-tZero : tm
-tSuc : tm -> tm
-tInd : tm -> (tm -> tm -> tm) -> tm -> tm
-tNat : tm
-tSig : tm -> (tm -> tm) -> tm
-tPack : tm -> tm -> tm
-tLet : tm -> (tm -> tm -> tm) -> tm
