theories/imports.v
@@ -9,6 +9,8 @@ Require Export Psatz.
 Global Set Warnings "-notation-overridden".
 Require Export Autosubst2.syntax.
 
+Scheme Equality for tm.
+
 Notation "s [ sigmatm ]" := (subst_tm sigmatm s) (at level 7, left associativity) : subst_scope.
 Notation "s ⟨ xitm ⟩" := (ren_tm xitm s) (at level 7, left associativity) : subst_scope.
 
