theories/typing_prop.v
@@ -1,0 +1,156 @@
+Require Import imports typing.
+
+Lemma Red_WtL Γ a b A (h : Γ ⊢ a ⤳ b ∈ A) : Γ ⊢ a ∈ A.
+Proof.
+  induction h; hauto lq:on ctrs:Wt.
+Qed.
+
+Lemma Reds_Wt Γ a b A (h : Γ ⊢ a ⤳* b ∈ A) : Γ ⊢ a ∈ A /\ Γ ⊢ b ∈ A.
+Proof. induction h; sfirstorder use:Red_WtL. Qed.
+
+Lemma here' : forall {A Γ T}, T = A ⟨shift⟩ ->  lookup 0 (A :: Γ) T.
+Proof. move => > ->. by apply here. Qed.
+
+Lemma there' : forall {n A Γ B T}, T = A ⟨shift⟩ ->
+      lookup n Γ A -> lookup (S n) (B :: Γ) T.
+Proof. move => > ->. by apply there. Qed.
+
+Lemma good_renaming_up ξ Γ Δ A :
+  lookup_good_renaming ξ Γ Δ ->
+  lookup_good_renaming (upRen_tm_tm ξ)  (A :: Γ) (A⟨ξ⟩ :: Δ).
+Proof.
+  rewrite /lookup_good_renaming => h.
+  move => i B.
+  inversion 1 =>*; subst.
+  - apply here'. by asimpl.
+  - asimpl. apply : there'; eauto. by asimpl.
+Qed.
+
+Lemma good_renaming_suc ξ Γ A Δ
+  (h : lookup_good_renaming ξ Γ Δ) :
+  lookup_good_renaming (ξ >> S) Γ (A⟨ξ⟩ :: Δ).
+Proof.
+  rewrite /lookup_good_renaming in h *.
+  move => i A0 /h ?.
+  asimpl. apply : there'; eauto. by asimpl.
+Qed.
+
+Lemma T_App' Γ a A B0 B b :
+  B0 = (subst_tm (b..) B) ->
+  Γ ⊢ a ∈ (tPi A B) ->
+  Γ ⊢ b ∈ A ->
+  (* -------------------- *)
+  Γ ⊢ (tApp a b) ∈ B0.
+Proof. move =>> ->. apply T_App. Qed.
+
+Lemma E_App' Γ a0 b0 a1 b1 A B T:
+  T = B[a0..] ->
+  Γ ⊢ b0 ≡ b1 ∈ tPi A B ->
+  Γ ⊢ a0 ≡ a1 ∈ A ->
+  (* ----------------- *)
+  Γ ⊢ tApp b0 a0 ≡ tApp b1 a1 ∈ T.
+Proof. move =>> ->. apply E_App. Qed.
+
+Lemma E_Beta' Γ A B a b i t T:
+  t = b[a..] ->
+  T = B[a..] ->
+  Γ ⊢ tPi A B ∈ tUniv i ->
+  A :: Γ ⊢ b ∈ B ->
+  Γ ⊢ a ∈ A ->
+  Γ ⊢ tApp (tAbs A b) a ≡ t ∈ T.
+Proof. move =>> -> ->. apply E_Beta. Qed.
+
+(* ------------------------------------- *)
+(* If a term is well-typed, then the context must be well-formed. *)
+
+Lemma Wt_Wff Γ a A (h : Γ ⊢ a ∈ A) : ⊢ Γ.
+Proof. elim : Γ a A / h => //. Qed.
+
+Lemma renaming_Syn_helper ξ a b C :
+  subst_tm (a ⟨ξ⟩ .: (b⟨ξ⟩)..) (ren_tm (upRen_tm_tm (upRen_tm_tm ξ)) C) = ren_tm ξ (subst_tm (a .: b ..) C).
+Proof. by asimpl. Qed.
+
+Lemma Wt_Univ Γ a A i
+  (h : Γ ⊢ a ∈ A) :
+  exists j, Γ ⊢ (tUniv i) ∈ (tUniv j).
+Proof.
+  exists (S i).
+  qauto l:on use:Wt_Wff ctrs:Wt.
+Qed.
+
+Lemma Wt_Pi_inv Γ A B U (h : Γ ⊢ (tPi A B) ∈ U) :
+  exists i, Γ ⊢ A ∈ (tUniv i) /\
+         (A :: Γ) ⊢ B ∈ (tUniv i).
+Proof.
+  move E : (tPi A B) h => T h.
+  move : A B E.
+  elim :  Γ T U / h => //.
+  - hauto lq:on use:Wt_Univ.
+Qed.
+
+Lemma renaming_wt_equiv :
+  (forall Γ a A, Γ ⊢ a ∈ A -> forall Δ ξ,
+    lookup_good_renaming ξ Γ Δ ->
+    ⊢ Δ ->  Δ ⊢ a⟨ξ⟩ ∈ A⟨ξ⟩) /\
+  (forall Γ a b A, Γ ⊢ a ≡ b ∈ A -> forall Δ ξ,
+    lookup_good_renaming ξ Γ Δ ->
+    ⊢ Δ ->  Δ ⊢ a⟨ξ⟩ ≡ b⟨ξ⟩ ∈ A⟨ξ⟩).
+Proof.
+  apply wt_mutual; try qauto l:on depth:1 ctrs:Wt,Equiv, lookup unfold:lookup_good_renaming.
+  - hauto q:on ctrs:Wt,Wff use:good_renaming_up.
+  - move => > _.
+    hauto q:on ctrs:Wt, Wff use:good_renaming_up, Wt_Pi_inv.
+  - move => * /=. apply : T_App'; eauto; by asimpl.
+  - hauto q:on ctrs:Wff,Equiv use:good_renaming_up.
+  - move => > + + _.
+    hauto q:on ctrs:Wt,Wff,Equiv use:good_renaming_up, Wt_Pi_inv.
+  - move => * /=. apply : E_App'; eauto; by asimpl.
+  - move => > _ * /=. apply : E_Beta'; eauto. by asimpl. by asimpl.
+    rewrite -/ren_tm.
+    hauto lq:on ctrs:Wff use:good_renaming_up, Wt_Pi_inv.
+Qed.
+
+Lemma renaming_wt : forall Γ a A, Γ ⊢ a ∈ A -> forall Δ ξ,
+    lookup_good_renaming ξ Γ Δ ->
+    ⊢ Δ ->  Δ ⊢ a⟨ξ⟩ ∈ A⟨ξ⟩.
+Proof. have := renaming_wt_equiv. tauto. Qed.
+
+Lemma renaming_wt_univ : forall Γ A i, Γ ⊢ A ∈ tUniv i -> forall Δ ξ,
+    lookup_good_renaming ξ Γ Δ ->
+    ⊢ Δ ->  Δ ⊢ A⟨ξ⟩ ∈ tUniv i.
+Proof. sfirstorder use:renaming_wt. Qed.
+
+Lemma renaming_equiv : forall Γ a b A, Γ ⊢ a ≡ b ∈ A -> forall Δ ξ,
+    lookup_good_renaming ξ Γ Δ ->
+    ⊢ Δ ->  Δ ⊢ a⟨ξ⟩ ≡ b⟨ξ⟩ ∈ A⟨ξ⟩.
+Proof. have := renaming_wt_equiv. tauto. Qed.
+
+Lemma R_App' Γ b0 b1 a A B T :
+  T = B[a..] ->
+  Γ ⊢ b0 ⤳ b1 ∈ tPi A B ->
+  Γ ⊢ a ∈ A ->
+  Γ ⊢ tApp b0 a ⤳ tApp b1 a ∈ T.
+Proof. move => ->. apply R_App. Qed.
+
+Lemma R_Beta' Γ A B a b i t T :
+  t = b[a..] ->
+  T = B[a..] ->
+  Γ ⊢ tPi A B ∈ tUniv i ->
+  A :: Γ ⊢ b ∈ B ->
+  Γ ⊢ a ∈ A ->
+  Γ ⊢ tApp (tAbs A b) a ⤳ t ∈ T.
+Proof. move => -> ->. apply R_Beta. Qed.
+
+Lemma renaming_Red Γ a b A (h : Γ ⊢ a ⤳ b ∈ A) : forall Δ ξ,
+    lookup_good_renaming ξ Γ Δ ->
+    ⊢ Δ ->  Δ ⊢ a⟨ξ⟩ ⤳ b⟨ξ⟩ ∈ A⟨ξ⟩.
+Proof.
+  elim : a b A / h.
+  - move => *. apply : R_App'; eauto using renaming_wt. by asimpl.
+  - move => A B a b i hPi hb ha Δ ξ hξ hΔ /=.
+    apply R_Beta' with (B := ren_tm (upRen_tm_tm ξ) B) (i := i); try by asimpl.
+    move /renaming_wt_univ : hPi. apply=>//.
+    have /= /Wt_Pi_inv : Δ ⊢  (tPi A B) ⟨ξ⟩ ∈ tUniv i by eauto using renaming_wt_univ.
+    hauto lq:on ctrs:Wt,Wff use:renaming_wt, good_renaming_up.
+    eauto using renaming_wt.
+Qed.
